HashToField: remove maxBits

Clap/HashToField.lean
@@ -9,17 +9,15 @@ open Clap.Lang
 abbrev p := Clap.Poseidon.p
 
 /-
-  `inputMaxbits` corresponds to the `{maxbits}` tag. Circom tags are assigned
-  values known at compile time.
+  There is a `{maxbits}` tag in keyless which seems to be set to 64.
 -/
 def hash64BitLimbsToField {numLimbs : ℕ}
-  (input : PaddedVector F p numLimbs)
-  (inputMaxbits : ℕ) :
+  (input : PaddedVector F p numLimbs) :
   Option (F p)
 :=
   let len := input.len
   let input := input.data
-  assert! inputMaxbits <= 64 && numLimbs != 0
+  assert! numLimbs != 0
   let w := (numLimbs + 2) / 3
   let padded : Vector (F p) (w * 3) :=
     have h : numLimbs ≤ w * 3 := by omega
@@ -104,14 +102,14 @@ example :
 
 example :
   -- poseidon [1, 2, 48]
-  hash64BitLimbsToField ⟨#v[1,0,0, 2,0,0],48⟩ 64 == some
+  hash64BitLimbsToField ⟨#v[1,0,0, 2,0,0],48⟩ == some
     9279947276585799077805428108942311632594603656807751900699542466687045499453
 := by
   native_decide
 
 example :
   -- poseidon [2^64, 24]
-  hash64BitLimbsToField ⟨#v[0,1,0],24⟩ 64 == some
+  hash64BitLimbsToField ⟨#v[0,1,0],24⟩ == some
     7782062960914706371652872958958905637393708115140004884697710811622618759288
 := by
   native_decide
